ImpMonads.v
@@ -2,26 +2,42 @@
 *)
 
 
-Require Import Program.
-
-
 Module Type MayReturnMonad.
 
+  (** The type of impure computations *)
   Axiom t: Type -> Type.
 
+  (** The may-return relation *)
   Axiom mayRet: forall {A:Type}, t A -> A -> Prop.
 
+  (** Standard monad operator: lift pure computation *)
   Axiom ret: forall {A}, A -> t A.
 
+  (** Standard monad operator: bind two impure computations *)
   Axiom bind: forall {A B}, (t A) -> (A -> t B) -> t B.
 
-  Axiom mk_annot: forall {A} (k: t A), t { a: A | mayRet k a }.
-
+  (** Axioms of monad operators wrt to may-return monad *)
   Axiom mayRet_ret: forall A (a b:A), 
      mayRet (ret a) b -> a=b.
 
   Axiom mayRet_bind: forall A B k1 k2 (b:B),
      mayRet (bind k1 k2) b -> exists a:A, mayRet k1 a /\ mayRet (k2 a) b.
+
+  (** Operator to annotate returned types with may-return relation.
+      This overcomes the non-dependent [bind] application within dependent types. 
+  *)
+  Axiom mk_annot: forall {A} (k: t A), t { a: A | mayRet k a }.
+
+  (** Exiting the monad for observationally deterministic computations (within partial correctness) *)
+  Axiom det_coerce: forall {A} (k: t A) (v: unit -> A) (DET: forall r, mayRet k r -> r = v tt), A.
+
+  Axiom det_coerce_correct: forall A (k: t A) v (DET: forall r, mayRet k r -> r = v tt), (det_coerce k v DET)=(v tt).
+
+  (** Exiting the monad on termination *)
+  Axiom has_returned: forall {A}, t A -> bool.
+
+  Axiom has_returned_correct: forall A (k: t A),
+     has_returned k = true -> exists r, mayRet k r.
 
 End MayReturnMonad.
 
@@ -29,7 +45,7 @@ End MayReturnMonad.
 
 (** Model of impure computation as predicate *)
 Module PowerSetMonad<: MayReturnMonad.
- 
+
    Definition t (A:Type) := A -> Prop.
 
    Definition mayRet {A:Type} (k: t A) a: Prop := k a.
@@ -52,8 +68,26 @@ Module PowerSetMonad<: MayReturnMonad.
      unfold mayRet, bind. 
      firstorder.
    Qed.
+  
+   (* exiting the monad: "logical" models *)
+
+   Definition det_coerce {A} (k: t A) (v: unit -> A) (DET: forall r, mayRet k r -> r = v tt) := v tt.
+
+   Lemma det_coerce_correct: forall A (k: t A) v (DET: forall r, mayRet k r -> r = v tt), det_coerce k v DET = v tt.
+   Proof.
+     unfold det_coerce; auto.
+   Qed.
+
+   Definition has_returned {A} (k:t A) := false.
+
+   Lemma has_returned_correct: forall A (k: t A),
+     has_returned k = true -> exists r, mayRet k r.
+   Proof.
+     unfold has_returned; congruence.
+   Qed.
 
 End PowerSetMonad.
+
 
 
 (** The identity interpretation *)
@@ -82,42 +116,106 @@ Module IdentityMonad<: MayReturnMonad.
      firstorder.
    Qed.
 
+   (* exiting the monad: "computational" models *)
+   Definition det_coerce {A} (k: t A) (v: unit -> A) (DET: forall r, mayRet k r -> r = v tt) := k.
+
+   Lemma det_coerce_correct A (k: t A) v (DET: forall r, mayRet k r -> r = v tt): det_coerce k v DET = v tt.
+   Proof.
+     eapply (DET k); refine (eq_refl _).
+     (* Very strange: in coq 8.16.1, "apply eq_refl" instead of "refine ..." generates a too strong universe constraint
+        that may later come problematic !
+     *)
+   Qed.
+
+   Definition has_returned {A} (k:t A) := true.
+
+   Lemma has_returned_correct: forall A (k: t A),
+     has_returned k = true -> exists r, mayRet k r.
+   Proof.
+     unfold has_returned, mayRet; eauto.
+   Qed.
+
 End IdentityMonad.
 
 
-(** Model of impure computation as state-transformers *)
-Module StateMonad<: MayReturnMonad.
+Require Program.
+
+(** Model of impure computation as state-transformers (with error-raising) *)
+Module StateOptionMonad<: MayReturnMonad.
  
    Parameter St: Type. (* A global state *)
 
-   Definition t (A:Type) := St -> A * St.
+   Definition t (A:Type) := St -> (option A) * St.
 
    Definition mayRet {A:Type} (k: t A) a: Prop :=
-     exists s, fst (k s)=a.
+     exists s, fst (k s)=Some a.
 
-   Definition ret {A:Type} (a:A) := fun (s:St) => (a,s).
+   Definition ret {A:Type} (a:A) := fun (s:St) => (Some a,s).
 
    Definition bind {A B:Type} (k1: t A) (k2: A -> t B) := 
-     fun s0 => let r := k1 s0 in k2 (fst r) (snd r).
+     fun s0 => 
+      let r := k1 s0 in 
+      match fst r with
+      | Some a => k2 a (snd r)
+      | None => (None, snd r)
+      end.
 
    Program Definition mk_annot {A} (k: t A) : t { a | mayRet k a } := 
-     fun s0 => let r := k s0 in (exist _ (fst r) _, snd r).
+     fun s0 =>
+     let r := k s0 in 
+     match fst r with
+     | Some a => (Some (exist _ a _), snd r)
+     | None => (None, snd r)
+     end.
    Obligation 1.
      unfold mayRet; eauto.
    Qed.
 
    Lemma mayRet_ret {A:Type} (a b:A): mayRet (ret a) b -> a=b.
    Proof.
-     unfold mayRet, ret. firstorder.
+     unfold mayRet, ret; simpl. firstorder congruence.
    Qed.
 
    Lemma mayRet_bind {A B:Type} k1 k2 (b:B):
          mayRet (bind k1 k2) b -> exists (a:A), mayRet k1 a /\ mayRet (k2 a) b.
    Proof.
-     unfold mayRet, bind. firstorder eauto.
-   Qed. 
+     unfold mayRet, bind.
+     intros (s & H); destruct (fst (k1 s)) eqn: H1; firstorder eauto.
+     simpl in *; congruence.
+   Qed.
 
-End StateMonad.
+   (* exiting the monad: "computational" models *)
+   Parameter st: St. (* the global state is not empty! *)
+
+   Definition det_coerce {A} (k: t A) (v: unit -> A) (DET: forall r, mayRet k r -> r = v tt): A 
+    := match fst (k st) with
+       | Some a => a
+       | None => v tt
+       end.
+
+   Lemma det_coerce_correct: forall A (k: t A) v (DET: forall r, mayRet k r -> r = v tt), det_coerce k v DET = v tt.
+   Proof.
+     unfold det_coerce, mayRet; intros A k v DET.
+     destruct (fst (k st)) eqn: H1; simpl; eauto.
+   Qed.
+
+   Definition has_returned {A} (k:t A) 
+   := match fst (k st) with
+      | Some _ => true
+      | None => false
+      end.
+
+   Lemma has_returned_correct: forall A (k: t A),
+     has_returned k = true -> exists r, mayRet k r.
+   Proof.
+     unfold has_returned, mayRet; intros A k H.
+     destruct (fst (k st)) eqn: H1; simpl; eauto.
+     congruence.
+   Qed.
+
+End StateOptionMonad.
+
+
 
 (** The deferred interpretation *)
 Module DeferredMonad<: MayReturnMonad.
@@ -143,6 +241,23 @@ Module DeferredMonad<: MayReturnMonad.
          mayRet (bind k1 k2) b -> exists (a:A), mayRet k1 a /\ mayRet (k2 a) b.
    Proof.
      firstorder.
+   Qed.
+
+   (* exiting the monad: "computational" models *)
+
+   Definition det_coerce {A} (k: t A) (v: unit -> A) (DET: forall r, mayRet k r -> r = v tt) := k tt.
+
+   Lemma det_coerce_correct: forall A (k: t A) v (DET: forall r, mayRet k r -> r = v tt), det_coerce k v DET = v tt.
+   Proof.
+     unfold det_coerce, mayRet; intros A k v DET; eapply DET. apply eq_refl.
+   Qed.
+
+   Definition has_returned {A} (k:t A) := true.
+
+   Lemma has_returned_correct: forall A (k: t A),
+     has_returned k = true -> exists r, mayRet k r.
+   Proof.
+     unfold has_returned, mayRet; eauto.
    Qed.
 
 End DeferredMonad.
