ImpPrelude.v
@@ -82,13 +82,13 @@ Qed.
 End PhysEqModel.
 
 Extract Inlined Constant phys_eq => "(==)".
-Hint Resolve phys_eq_correct: wlp.
+#[global] Hint Resolve phys_eq_correct: wlp.
 
 
 Axiom struct_eq: forall {A}, A -> A -> ?? bool.
 Axiom struct_eq_correct: forall A (x y:A), WHEN struct_eq x y ~> b THEN if b then x=y else x<>y.
 Extract Inlined Constant struct_eq => "(=)".
-Hint Resolve struct_eq_correct: wlp.
+#[global] Hint Resolve struct_eq_correct: wlp.
 
 
 (** Data-structure for generic hash-consing *)
